README.md
@@ -1,2 +1,5 @@
 # coqstlczk
 Coq proofs for ZK proof compilers
+
+## Requirements
+coq-bignums library.
